more

haskell/thih/Syntax.hs
@@ -1,0 +1,67 @@
+type Id = String
+
+enumId :: Int -> Id
+enumId n = "v" ++ show n
+
+data Kind = Star | Kfun Kind Kind deriving Eq
+
+data Tyvar = Tyvar Id Kind deriving Eq
+
+data Tycon = Tycon Id Kind deriving Eq
+
+data Type = TVar Tyvar | TCon Tycon | TAp Type Type | TGen Int deriving Eq
+
+tUnit    :: Type 
+tChar    :: Type 
+tInt     :: Type 
+tInteger :: Type 
+tFloat   :: Type 
+tDouble  :: Type 
+tList    :: Type 
+tArrow   :: Type 
+tTuple2  :: Type 
+tString  :: Type
+ 
+tUnit    = TCon (Tycon "()" Star)
+tChar    = TCon (Tycon "Char" Star)
+tInt     = TCon (Tycon "Int" Star)
+tInteger = TCon (Tycon "Integer" Star)
+tFloat   = TCon (Tycon "Float" Star)
+tDouble  = TCon (Tycon "Double" Star)
+tString  = list tChar   
+
+
+tList    = TCon (Tycon "[]" (Kfun Star Star))
+tArrow   = TCon (Tycon "(->)" (Kfun Star (Kfun Star Star)))
+tTuple2  = TCon (Tycon "(,)"  (Kfun Star (Kfun Star Star)))
+
+infixr 4 `fn`
+
+fn :: Type -> Type -> Type 
+a `fn` b = TAp (TAp tArrow a) b
+
+list :: Type -> Type
+list a = TAp tList a
+
+pair :: Type -> Type -> Type
+pair a b = TAp (TAp tTuple2 a) b
+
+class HasKind t where
+    kind :: t -> Kind
+
+instance HasKind Tyvar where
+    kind (Tyvar _ k) = k
+
+instance HasKind Tycon where
+    kind (Tycon _ k) = k
+
+instance HasKind Type where
+    kind (TCon tycon) = kind tycon
+    kind (TVar tyvar) = kind tyvar
+    kind (TGen _)     = error "kind : TGen type has unknown kind" 
+    kind (TAp a b)    = case kind a of 
+        Kfun k1 k2   -> if kind b == k1 then k2 else error "kind : kind mismatch"
+        _            -> error "kind : a is *"
+
+
+
