coq/cpdt/nested_ind.v
@@ -1,3 +1,5 @@
+Require Import List.
+
 (* We are using the type we are defining as the argument of 
    parameterized type family: this is a nested inductive type
 *)
@@ -60,7 +62,21 @@ Fixpoint tree_nested_ind (a:Set) (P:tree a -> Prop)
                 end) ts)
         end.
 
+Lemma tree_nested_ind2 : forall (a:Set) (P:tree a-> Prop),
+    (forall (x:a), P (Node x nil)) ->
+    (forall (x:a) (t:tree a) (ts:list (tree a)), P t -> P (Node x ts) -> P (Node x (t :: ts))) ->
+    forall (t:tree a), P t.
+Proof.
+    intros a P Hnil Hcons.
+    apply tree_nested_ind. intros x. induction ts as [|t ts IH].
+    - intros. apply Hnil.
+    - intros [H0 H1]. apply Hcons.
+        + assumption.
+        + apply IH. assumption.
+Qed.
 
+
+(* This has nothing to do with 'tree a' but used here to illustrate a point *) 
 Fixpoint map (a b:Set) (f:a -> b) (xs:list a) : list b :=
     match xs with
     | nil       => nil
@@ -69,7 +85,7 @@ Fixpoint map (a b:Set) (f:a -> b) (xs:list a) : list b :=
 
 Arguments map {a} {b} _ _.
 
-(* This fails despite looking very legitimate
+(* This 'map'-based solution fails despite looking very legitimate
 Fixpoint fmap (a b:Set) (f:a -> b) (t:tree a) {struct t} : tree b :=
     match t with
     | Node x ts     => Node (f x) (map (fmap a b f) ts) 
@@ -90,23 +106,42 @@ Fixpoint fmap (a b:Set) (f:a -> b) (t:tree a) : tree b :=
 
 Arguments fmap {a} {b} _ _. 
 
-Definition g (a b:Set) (f:a -> b) (t:tree a) : tree b :=
+Lemma fmap_check1 : forall (a b:Set) (f:a -> b) (x:a), 
+    fmap f (Node x nil) = Node (f x) nil.
+Proof. intros  a b f x. reflexivity. Qed.
+
+
+Definition extract (a:Set) (t:tree a) : list (tree a) :=
     match t with
-    | Node x ts     => Node (f x) (map (fmap f) ts)
+    | Node _ ts     => ts
     end.
 
-Arguments g {a} {b} _ _.
+Arguments extract {a} _.
 
-Lemma fmap_check : forall (a b:Set) (f:a -> b) (t:tree a),
-    fmap f t = g f t.
+Lemma extract_fmap : forall (a b:Set) (f:a -> b) (t:tree a),
+    extract (fmap f t) = map (fmap f) (extract t).
 Proof.
-    intros a b f. apply (tree_nested_ind a
-        (fun (t:tree a) => fmap f t = g f t)).
-    intros x ts. induction ts as [|t ts IH].
-    - reflexivity.
-    - intros [H1 H2]. apply IH in H2.
+    intros a b f. apply tree_nested_ind2.
+    - intros x. reflexivity.
+    - intros x t ts H0 H1. simpl. unfold map. reflexivity.
+
 Show.
 
+
+(*
+Lemma fmap_check2 : forall (a b:Set) (f:a -> b) (x:a) (ts:list (tree a)),
+    fmap f (Node x ts) = Node (f x) (map (fmap f) ts).
+Proof.
+    intros a b f x ts. remember (Node x ts) as t eqn:H. revert x ts H.
+    apply (tree_nested_ind2 a (fun t =>
+        forall (x : a) (ts : list (tree a)), t = Node x ts -> 
+            fmap f t = Node (f x) (map (fmap f) ts))).
+    - intros x y ts H. injection H. intros. subst. reflexivity.
+    - clear t. intros x t ts H0 H1 y ts' H2. injection H2. intros. subst.
+      
+
+Show.
+*)
 
 (*
 (* Another failure, leading to nested recursion
@@ -164,4 +199,3 @@ Proof. intros a b f t.
        - intros H. destruct H as [H1 H2]. apply IH in H2.
 Show.
 *)
-
